theories/cancellation/ElimRel.v
@@ -65,14 +65,14 @@ End CancelLib.
 Section ELIM_REL.
 Context `{_crisG: !crisG Γ Σ α β τ _S _I, _concG: !concG}.
 
-Definition HoareSpawnE (fspo: option fspec) (sspo: bool) fn varg N : itree crisE nat :=
+Definition HoareSpawnE (fspo: option fspec) (sspo: bool) fn varg : itree crisE nat :=
   match fspo, sspo with
   | Some fsp, true =>
       x <- trigger (Choose (meta fsp));; tau;;
       arg <- trigger (Choose Any.t);; tau;;
       tid <- trigger (Spawn fn arg);; tau;;
       trigger (Assume (YIELD tid));;; tau;;
-      trigger (Guarantee (YIELD tid -∗ TID tid -∗ winv (↑N, ↑N) -∗ precond fsp (N, tid) x varg arg));;; tau;;
+      trigger (Guarantee (YIELD tid -∗ TID tid -∗ winv (⊤, ⊤) -∗ precond fsp x varg arg));;; tau;;
       Ret tid
   | None, true =>
       tid <- trigger (Spawn fn varg);; tau;;
@@ -83,23 +83,25 @@ Definition HoareSpawnE (fspo: option fspec) (sspo: bool) fn varg N : itree crisE
       Ret tid
   end.
 
-Definition HoareYieldE (sspo: bool) N stid ntid : itree crisE () :=
+Definition HoareYieldE (sspo: bool) ntid : itree crisE () :=
   if sspo
   then
-      trigger (Guarantee (TID stid ∗ YIELD ntid ∗ winv (↑N, ↑N)));;; tau;;
+      stid <- trigger (Choose nat);; tau;;
+      trigger (Guarantee (TID stid ∗ YIELD ntid ∗ winv (⊤, ⊤)));;; tau;;
       trigger (Yield ntid);;; tau;;
-      trigger (Assume (TID stid ∗ YIELD stid ∗ winv (↑N, ↑N)));;; tau;;
+      trigger (Assume (TID stid ∗ YIELD stid ∗ winv (⊤, ⊤)));;; tau;;
       Ret tt
   else
       trigger (Yield ntid);;; tau;; Ret tt.
 
-Lemma HoareYieldE_indep N0 N1 stid0 stid1 ntid :
+(* Lemma HoareYieldE_indep N0 N1 stid0 stid1 ntid :
   HoareYieldE false N0 stid0 ntid = HoareYieldE false N1 stid1 ntid.
-Proof using. ss. Qed.
+Proof using. ss. Qed. *)
 
-Definition HoareGetTidE (sspo: bool) stid : itree crisE nat :=
+Definition HoareGetTidE (sspo: bool) : itree crisE nat :=
   if sspo
   then
+      stid <- trigger (Choose nat);; tau;;
       trigger (Guarantee (TID(stid)));;; tau;;
       tid <- trigger GetTid;; tau;;
       trigger (Assume (⌜tid = stid⌝ ∗ TID(stid)));;; tau;;
@@ -107,29 +109,28 @@ Definition HoareGetTidE (sspo: bool) stid : itree crisE nat :=
   else
       tid <- trigger GetTid;; tau;; Ret tid.
 
-Lemma HoareGetTidE_indep stid0 stid1 :
+(* Lemma HoareGetTidE_indep stid0 stid1 :
   HoareGetTidE false stid0 = HoareGetTidE false stid1.
-Proof using. ss. Qed.
+Proof using. ss. Qed. *)
 
-Definition elim_precond {X X' : Type} P P' (N: namespace) (stid: nat) (varg: Any.t) : itree crisE (namespace * nat * X * X' * Any.t) :=
+Definition elim_precond {X X' : Type} P P' (varg: Any.t) : itree crisE (X * X' * Any.t) :=
   x <- trigger (Choose X);; tau;;
   arg <- trigger (Choose Any.t);; tau;;
   (* trigger (Guarantee (TID stid ∗ YIELD stid ∗ winv (↑N, ↑N)));;; tau;; *)
-  trigger (Guarantee (P (N, stid) x varg arg));;; tau;; tau;;
-  '(N', stid') : _ <- trigger (Take (namespace * nat));; tau;;
+  trigger (Guarantee (P x varg arg));;; tau;; tau;;
   x' <- trigger (Take X');; tau;;
   varg' <- trigger (Take Any.t);; tau;;
   (* trigger (Assume (TID stid' ∗ YIELD stid' ∗ winv (↑(N'), ↑(N'))));;; tau;; *)
-  trigger (Assume (P' (N', stid') x' varg' arg));;; tau;;
-  Ret (N', stid', x, x', varg').
+  trigger (Assume (P' x' varg' arg));;; tau;;
+  Ret (x, x', varg').
 
-Definition elim_postcond {X X' : Type} Q Q' (N N': namespace) (stid stid': nat) (x : X) (x' : X') (vret': Any.t) : itree crisE Any.t :=
+Definition elim_postcond {X X' : Type} Q Q' (x : X) (x' : X') (vret': Any.t) : itree crisE Any.t :=
   ret <- trigger (Choose Any.t);; tau;;
   (* trigger (Guarantee (TID stid' ∗ YIELD stid' ∗ winv (↑N', ↑N')));;; tau;; *)
-  trigger (Guarantee (Q' (N', stid') x' vret' ret));;; tau;; tau;; tau;;
+  trigger (Guarantee (Q' x' vret' ret));;; tau;; tau;; tau;;
   vret <- trigger (Take Any.t);; tau;;
   (* trigger (Assume (TID stid ∗ YIELD stid ∗ winv (↑N, ↑N)));;; tau;; *)
-  trigger (Assume (Q (N, stid) x vret ret));;; tau;;
+  trigger (Assume (Q x vret ret));;; tau;;
   Ret vret.
 
 (* Definition elim_trivial_precond (arg: Any.t) : itree crisE Any.t := *)
@@ -143,81 +144,80 @@ Definition elim_postcond {X X' : Type} Q Q' (N N': namespace) (stid stid': nat) 
 (*   trigger (Guarantee (⌜vret = ret⌝)%I);;; tau;; *)
 (*   Ret ret. *)
 
-Definition elim_spawnee_precond (X : Type) P (arg : Any.t) : itree crisE (namespace * nat * X * Any.t) :=
-  '(N, stid) : _ <- trigger (Take (namespace * nat));; tau;;
+Definition elim_spawnee_precond (X : Type) P (arg : Any.t) : itree crisE (X * Any.t) :=
   x <- trigger (Take X);; tau;;
   varg <- trigger (Take Any.t);; tau;;
   (* trigger (Assume (TID stid ∗ YIELD stid ∗ winv (↑N, ↑N)));;; tau;; *)
-  trigger (Assume (P (N, stid) x varg arg));;; tau;;
-  Ret (N, stid, x, varg).
+  trigger (Assume (P x varg arg));;; tau;;
+  Ret (x, varg).
 
-Definition elim_spawnee_postcond {X : Type} Q (N: namespace) (stid : nat) (x : X) (vret : Any.t) : itree crisE Any.t :=
+Definition elim_spawnee_postcond {X : Type} Q (x : X) (vret : Any.t) : itree crisE Any.t :=
   ret <- trigger (Choose Any.t);; tau;;
   (* trigger (Guarantee (TID stid ∗ YIELD stid ∗ winv (↑N, ↑N)));;; tau;; *)
-  trigger (Guarantee (Q (N, stid) x vret ret));;; tau;;
+  trigger (Guarantee (Q x vret ret));;; tau;;
   Ret ret.
 
 Variant elim_rel_def
-    (N: namespace) (sp : specmap)
+    (sp : specmap)
     (self : ∀ T, Σ → itree crisE T → itree crisE T → Prop) (T : Type)
   : Σ → itree crisE T → itree crisE T → Prop :=
 
 (* handling void cases *)
 | elim_take_false ktrS itrT :
-   elim_rel_def N sp self ε (trigger (Take False) >>= ktrS) itrT
+   elim_rel_def sp self ε (trigger (Take False) >>= ktrS) itrT
 | elim_tau_take_false ktrS itrT :
-   elim_rel_def N sp self ε (tau;; trigger (Take False) >>= ktrS) itrT
+   elim_rel_def sp self ε (tau;; trigger (Take False) >>= ktrS) itrT
 | elim_choose_false itrS ktrT :
-   elim_rel_def N sp self ε itrS (trigger (Choose False) >>= ktrT)
+   elim_rel_def sp self ε itrS (trigger (Choose False) >>= ktrT)
 (* handling normal cases *)
 | elim_rel_ret v :
-   elim_rel_def N sp self ε (Ret v) (Ret v)
+   elim_rel_def sp self ε (Ret v) (Ret v)
 | elim_rel_tau itrS itrT :
    self _ ε itrS itrT →
-   elim_rel_def N sp self ε (tau;; itrS) (tau;; itrT)
+   elim_rel_def sp self ε (tau;; itrS) (tau;; itrT)
 | elim_rel_core {R} (e : coreE R) ktrS ktrT :
    (∀ (x : R), self _ ε (ktrS x) (ktrT x)) →
-   elim_rel_def N sp self ε (trigger e >>= ktrS) (a <- trigger e;; ktrT a)
+   elim_rel_def sp self ε (trigger e >>= ktrS) (a <- trigger e;; ktrT a)
 | elim_rel_pg {R} (e : pgE R) ktrS ktrT :
    (∀ (x : R), self _ ε (ktrS x) (ktrT x)) →
-   elim_rel_def N sp self ε (trigger e >>= ktrS) (a <- trigger e;; ktrT a)
+   elim_rel_def sp self ε (trigger e >>= ktrS) (a <- trigger e;; ktrT a)
 | elim_rel_ag {R} (e : agE R) ktrS ktrT :
    (∀ (x : R), self _ ε (ktrS x) (ktrT x)) →
-   elim_rel_def N sp self ε (trigger e >>= ktrS) (a <- trigger e;; ktrT a)
+   elim_rel_def sp self ε (trigger e >>= ktrS) (a <- trigger e;; ktrT a)
 (* handling cancellation *)
-| elim_rel_yield tid ntid ktrS ktrT itrS itrT :
-    itrS = HoareYieldE false N tid ntid >>= ktrS →
-    itrT = HoareYieldE true N tid ntid >>= ktrT →
+| elim_rel_yield ntid ktrS ktrT itrS itrT :
+    itrS = HoareYieldE false ntid >>= ktrS →
+    itrT = HoareYieldE true ntid >>= ktrT →
     (∀ x, self _ ε (ktrS x) (ktrT x)) →
-    elim_rel_def N sp self ε itrS itrT
+    elim_rel_def sp self ε itrS itrT
 | elim_rel_spawn fn args ktrS ktrT itrS itrT :
    (* (img = false → fspec_imply (fspec_flat (sp fn)) fspec_trivial) → *)
-   itrS = HoareSpawnE None false fn args N >>= ktrS →
-   itrT = HoareSpawnE (sp !! (speckey_fn fn)) true fn args N >>= ktrT →
+   itrS = HoareSpawnE None false fn args >>= ktrS →
+   itrT = HoareSpawnE (sp !! (speckey_fn fn)) true fn args >>= ktrT →
    (∀ x, self _ ε (ktrS x) (ktrT x)) →
-   elim_rel_def N sp self ε itrS itrT
-| elim_rel_precond (X X' : Type) P P' stid varg itrS itrT ktrT :
+   elim_rel_def sp self ε itrS itrT
+| elim_rel_precond (X X' : Type) P P' varg itrS itrT ktrT :
    (∀ (x : X), ∃ (x' : X'),
-     (∀ arg, P (N, stid) x varg arg ⊢ |==> P' (N, stid) x' varg arg) ∧ self _ ε itrS (ktrT (N, stid, x, x', varg))) →
-   itrT = elim_precond P P' N stid varg >>= ktrT →
-   elim_rel_def N sp self ε (tau;; tau;; tau;; itrS) itrT
-| elim_rel_postcond (X X': Type) Q Q' (stid: nat) (x: X) (x': X') vret itrS itrT ktrT :
-   ((∀ ret, Q' (N, stid) x' vret ret ⊢ |==> Q (N, stid) x vret ret) ∧ self _ ε itrS (ktrT vret)) →
-   itrT = elim_postcond Q Q' N N stid stid x x' vret >>= ktrT →
-   elim_rel_def N sp self ε (tau;; tau;; itrS) itrT
-| elim_rel_gettid tid ktrS ktrT itrS itrT :
-   itrS = HoareGetTidE false tid >>= ktrS ->
-   itrT = HoareGetTidE true tid >>= ktrT ->
+     (∀ arg, P x varg arg ⊢ |==> P' x' varg arg) ∧ self _ ε itrS (ktrT (x, x', varg))) →
+   itrT = elim_precond P P' varg >>= ktrT →
+   elim_rel_def sp self ε (tau;; tau;; tau;; itrS) itrT
+| elim_rel_postcond (X X': Type) Q Q' (x: X) (x': X') vret itrS itrT ktrT :
+   ((∀ ret, Q' x' vret ret ⊢ |==> Q x vret ret) ∧ self _ ε itrS (ktrT vret)) →
+   itrT = elim_postcond Q Q' x x' vret >>= ktrT →
+   elim_rel_def sp self ε (tau;; tau;; itrS) itrT
+| elim_rel_gettid ktrS ktrT itrS itrT :
+   itrS = HoareGetTidE false >>= ktrS ->
+   itrT = HoareGetTidE true >>= ktrT ->
    (∀ x, self _ ε (ktrS x) (ktrT x)) ->
-   elim_rel_def N sp self ε itrS itrT
+   elim_rel_def sp self ε itrS itrT
 .
 
-Definition elim_rel N sp T r_diff itrS itrT :=
-  paco4 (@elim_rel_def N sp) bot4 T r_diff itrS itrT.
+Definition elim_rel sp T r_diff itrS itrT :=
+  paco4 (@elim_rel_def sp) bot4 T r_diff itrS itrT.
 
-Lemma elim_rel_def_mon N sp r1 r2 :
+Lemma elim_rel_def_mon sp r1 r2 :
   r1 <4= r2 →
-  @elim_rel_def N sp r1 <4= elim_rel_def N sp r2.
+  @elim_rel_def sp r1 <4= elim_rel_def sp r2.
 Proof using.
   intros ??????PR; destruct PR; eauto using @elim_rel_def.
   - eapply elim_rel_precond; eauto; des_safe.
@@ -240,13 +240,13 @@ Variant elim_rel_bindC
 Lemma elim_rel_bindC_mon : monotone4 elim_rel_bindC.
 Proof using. ii. destruct IN; econs; eauto. Qed.
 
-Lemma elim_rel_bindC_spec N sp :
-  elim_rel_bindC <5= gupaco4 (@elim_rel_def N sp) (cpn4 (@elim_rel_def N sp)).
+Lemma elim_rel_bindC_spec sp :
+  elim_rel_bindC <5= gupaco4 (@elim_rel_def sp) (cpn4 (@elim_rel_def sp)).
 Proof using.
   eapply wrespect4_uclo; eauto with paco.
   econs; [apply elim_rel_bindC_mon|].
   i. inv PR. apply GF in H.
-  inv H; grind; eauto 7 using rclo4, elim_rel_def, elim_rel_bindC with paco.
+  inv H; grind; eauto 6 using rclo4, elim_rel_def, elim_rel_bindC with paco.
   - ired. eapply elim_rel_yield with (ktrS := λ z, (x <- ktrS0 z;; ktrS x)) (ktrT := λ z, (x <- ktrT0 z;; ktrT x)); eauto.
     { ired; ss. } { ired; ss. }
     eauto 7 using rclo4, elim_rel_def, elim_rel_bindC with paco.
@@ -279,12 +279,12 @@ Proof using.
   { rewrite /triggerUB. ss. rewrite vis_trigger. f_equal. extensionalities. ss. }
 Qed.
 
-Lemma SBRed_HoareSpawn (msk : emask) fn varg sspo fspo N
+Lemma SBRed_HoareSpawn (msk : emask) fn varg sspo fspo
   (MSK: ∀ x, msk _ (subevent _ (Spawn fn x)) = true)
   (IMG: img_msk msk)
   :
-  SB.sandbox msk (SModTr.HoareSpawn fspo sspo fn varg N) =
-    SModTr.HoareSpawn fspo sspo fn varg N.
+  SB.sandbox msk (SModTr.HoareSpawn fspo sspo fn varg) =
+    SModTr.HoareSpawn fspo sspo fn varg.
 Proof using.
   r in IMG; des.
   rewrite /SModTr.HoareSpawn. destruct fspo, sspo; cycle 1.
@@ -307,8 +307,8 @@ Proof using.
   rewrite SBRed.ret bind_ret_l. rewrite SBRed.ret //.
 Qed.
 
-Lemma MIRed_HoareSpawn prog fspo sspo fn varg N :
-  inline_body prog (SModTr.HoareSpawn fspo sspo fn varg N) = HoareSpawnE fspo sspo fn varg N.
+Lemma MIRed_HoareSpawn prog fspo sspo fn varg :
+  inline_body prog (SModTr.HoareSpawn fspo sspo fn varg) = HoareSpawnE fspo sspo fn varg.
 Proof using.
   destruct sspo; ss; cycle 1.
   { destruct fspo; ss; cycle 1.
@@ -331,48 +331,51 @@ Proof using.
   by rewrite MIRed.ret.
 Qed.
 
-Lemma SBRed_HoareYield (msk: emask) sspo N stid ntid
+Lemma SBRed_HoareYield (msk: emask) sspo ntid
   (MSK: msk _ (subevent _ (Yield ntid)) = true)
   (IMG: img_msk msk) :
-  SB.sandbox msk (SModTr.HoareYield sspo N stid ntid) =
-    SModTr.HoareYield sspo N stid ntid.
+  SB.sandbox msk (SModTr.HoareYield sspo ntid) =
+    SModTr.HoareYield sspo ntid.
 Proof using.
   r in IMG; des.
   rewrite /SModTr.HoareYield. destruct sspo; cycle 1.
   { rewrite SBRed.vis MSK vis_trigger. rewrite -{2}(bind_ret_r (trigger (Yield _))).
     f_equal. extensionalities. rewrite SBRed.ret //. }
-  rewrite SBRed.bind SBRed.vis IMG3 vis_trigger. ired. f_equal. extensionalities.
-  rewrite SBRed.ret bind_ret_l.
-  rewrite SBRed.bind SBRed.vis MSK vis_trigger. ired. f_equal. extensionalities.
-  rewrite SBRed.ret bind_ret_l.
-  rewrite SBRed.vis IMG1 vis_trigger -{2}(bind_ret_r (trigger (Assume _))). f_equal. extensionalities.
+  etrans; [hnorm_itr|]; rewrite IMG0; etrans; [hnorm_itr|]; grind.
+  etrans; [hnorm_itr|]; rewrite IMG3; etrans; [hnorm_itr|]; grind.
+  etrans; [hnorm_itr|]; rewrite MSK; etrans; [hnorm_itr|]; grind.
+  etrans; [hnorm_itr|]; rewrite IMG1; etrans; [hnorm_itr|]; grind.
+  rewrite -{2}(bind_ret_r (trigger (Assume _))). f_equal. extensionalities.
   rewrite SBRed.ret //.
 Qed.
 
-Lemma MIRed_HoareYield prog sspo N stid ntid :
-  inline_body prog (SModTr.HoareYield sspo N stid ntid) = HoareYieldE sspo N stid ntid.
+Lemma MIRed_HoareYield prog sspo ntid :
+  inline_body prog (SModTr.HoareYield sspo ntid) = HoareYieldE sspo ntid.
 Proof using.
   rewrite /SModTr.HoareYield /HoareYieldE. destruct sspo; cycle 1.
   { rewrite -{1}(bind_ret_r (trigger (Yield _))) MIRed.yield.
     f_equal. extensionalities. do 2 f_equal. rewrite MIRed.ret.
     by destruct H. }
+  rewrite MIRed.core. f_equal. extensionalities. do 2 f_equal.  
   rewrite MIRed.ag. f_equal. extensionalities. do 2 f_equal.
   rewrite MIRed.yield. f_equal. extensionalities. do 2 f_equal.
   rewrite -{1}(bind_ret_r (trigger _)).
   rewrite MIRed.ag. f_equal. extensionalities. do 2 f_equal.
-  destruct H1. by rewrite MIRed.ret.
+  destruct H2. by rewrite MIRed.ret.
 Qed.
 
-Lemma SBRed_HoareGetTid (msk : emask) sspo stid
+Lemma SBRed_HoareGetTid (msk : emask) sspo
   (MSK: msk _ (subevent _ GetTid) = true)
   (IMG: img_msk msk) :
-  SB.sandbox msk (SModTr.HoareGetTid sspo stid) =
-    SModTr.HoareGetTid sspo stid.
+  SB.sandbox msk (SModTr.HoareGetTid sspo) =
+    SModTr.HoareGetTid sspo.
 Proof using.
   r in IMG. des.
   rewrite /SModTr.HoareGetTid. destruct sspo; cycle 1.
   { rewrite SBRed.vis MSK vis_trigger. rewrite -{2}(bind_ret_r (trigger _)).
     f_equal. extensionalities. rewrite SBRed.ret //. }
+  rewrite SBRed.bind SBRed.vis IMG0 vis_trigger bind_bind. f_equal. extensionalities.
+  rewrite SBRed.ret bind_ret_l.
   rewrite SBRed.bind SBRed.vis IMG3 vis_trigger bind_bind. f_equal. extensionalities.
   rewrite SBRed.ret bind_ret_l.
   rewrite SBRed.bind SBRed.vis MSK vis_trigger bind_bind. f_equal. extensionalities.
@@ -382,13 +385,14 @@ Proof using.
   rewrite SBRed.ret //.
 Qed.
 
-Lemma MIRed_HoareGetTid prog sspo stid :
-  inline_body prog (SModTr.HoareGetTid sspo stid) = HoareGetTidE sspo stid.
+Lemma MIRed_HoareGetTid prog sspo :
+  inline_body prog (SModTr.HoareGetTid sspo) = HoareGetTidE sspo.
 Proof using.
   rewrite /SModTr.HoareGetTid /HoareGetTidE. destruct sspo; cycle 1.
   { rewrite -{1}(bind_ret_r (trigger GetTid)) MIRed.gettid.
     f_equal. extensionalities. do 2 f_equal. rewrite MIRed.ret.
     by destruct H. }
+  rewrite MIRed.core. f_equal. extensionalities. do 2 f_equal.
   rewrite MIRed.ag. f_equal. extensionalities. do 2 f_equal.
   rewrite MIRed.gettid. f_equal. extensionalities. do 2 f_equal.
   rewrite MIRed.ag. f_equal. extensionalities. do 2 f_equal.
@@ -408,22 +412,18 @@ Lemma MIRed_HoareFun
   fspo = Some (@fspec_mk _ meta pre post) →
   inline_body
     (sandboxed_prog (SMod.to_mod sp md))
-    (SB.sandbox_body (msk, SModTr.HoareFun fspo (λ N tid, (SModTr.trans sp N tid ∘ bd))) arg) =
-  '(N, tid, x, varg) : _ <- @elim_spawnee_precond _ pre arg;;
+    (SB.sandbox_body (msk, SModTr.HoareFun fspo (SModTr.trans sp ∘ bd)) arg) =
+  '(x, varg) : _ <- @elim_spawnee_precond _ pre arg;;
   vret <-
     inline_body
       (sandboxed_prog (SMod.to_mod sp md))
-      (SB.sandbox msk (SModTr.trans sp N tid (bd varg)));;
-  elim_spawnee_postcond post N tid x vret.
+      (SB.sandbox msk (SModTr.trans sp (bd varg)));;
+  elim_spawnee_postcond post x vret.
 Proof using.
   intros Hfind Himg Hst. r in Himg. des.
   rewrite /SModTr.HoareFun /elim_spawnee_precond /elim_spawnee_postcond /=.
   destruct fspo; ss. destruct f; ss. depdes Hst.
   rewrite /SB.sandbox_body SBRed.bind SBRed.vis /= Himg vis_trigger !bind_bind MIRed.core.
-  ired; f_equal. extensionalities x; ired; do 2 f_equal.
-  destruct x. ired. do 2 f_equal.
-  rewrite SBRed.ret bind_ret_l.
-  rewrite SBRed.bind SBRed.vis /= Himg vis_trigger !bind_bind MIRed.core.
   ired; f_equal. extensionalities x; ired; do 2 f_equal.
   rewrite SBRed.ret bind_ret_l.
   rewrite SBRed.bind SBRed.vis /= Himg vis_trigger !bind_bind MIRed.core.
@@ -451,7 +451,7 @@ Proof using.
 Qed.
 
 Lemma MIRed_HoareCall md sp fn varg
-  (msk msk0: emask) fspo fspo0 bd0 m m0 pre pre0 post post0 N stid
+  (msk msk0: emask) fspo fspo0 bd0 m m0 pre pre0 post post0
   (WF: SMod.cancellable md)
   (* (SPWF: speckey_concE ∈ dom sp) *)
   (IN: ∀ x, msk _ (subevent _ (Call fn x)) = true)
@@ -461,15 +461,15 @@ Lemma MIRed_HoareCall md sp fn varg
   (ST: fspo = Some (@fspec_mk _ m pre post))
   (ST0: fspo0 = Some (@fspec_mk _ m0 pre0 post0))
   :
-  inline_body (sandboxed_prog (SMod.to_mod sp md)) (SB.sandbox msk (SModTr.HoareCall fspo fn varg N stid))
+  inline_body (sandboxed_prog (SMod.to_mod sp md)) (SB.sandbox msk (SModTr.HoareCall fspo fn varg))
   =
   (* head *)
-  '(N', stid', x,x0,arg):_ <- elim_precond pre pre0 N stid varg ;;
+  '(x, x0,arg):_ <- elim_precond pre pre0 varg ;;
   (* body *)
   vret0 <- inline_body (sandboxed_prog (SMod.to_mod sp md)) 
-                       (SB.sandbox msk0 (SModTr.trans sp N' stid' (bd0 arg)));;
+                       (SB.sandbox msk0 (SModTr.trans sp (bd0 arg)));;
   (* tail *)
-  elim_postcond post post0 N N' stid stid' x x0 vret0.
+  elim_postcond post post0 x x0 vret0.
 Proof using.
   r in IMG. des.
   r in WF. hexploit WF; eauto. intros [IM [_ _]]. r in IM. des.
@@ -492,10 +492,7 @@ Proof using.
   rewrite {2}/sandboxed_prog. rewrite lookup_omap {2}/SMod.to_mod /= lookup_fmap FIND /= bind_ret_l.
   rewrite /SB.sandbox_body /SModTr.trans_fnsem. s.
   rewrite !SBRed.bind SBRed.vis /= IM vis_trigger !bind_bind MIRed.core. do 2 f_equal.
-  extensionalities. ired. destruct H2. ired. do 2 f_equal.
-  rewrite !SBRed.ret bind_ret_l.
-  rewrite !SBRed.bind !SBRed.vis /= IM vis_trigger !bind_bind MIRed.core. do 2 f_equal.
-  extensionalities. ired. do 2 f_equal.
+  extensionalities. ired. destruct H1. ired. do 2 f_equal.
   rewrite !SBRed.ret bind_ret_l.
   rewrite !SBRed.bind !SBRed.vis /= IM vis_trigger !bind_bind MIRed.core. do 2 f_equal.
   extensionalities. ired. do 2 f_equal.
@@ -531,18 +528,18 @@ Proof using.
 Local Tactic Notation "estep" integer(n) := do n (gstep; econs; i).
 Local Ltac edone := eauto 6 with paco.
 
-Lemma elim_rel_cancel (md: SMod.t) T msk sN tN stid ttid (itr: itree _ T)
+Lemma elim_rel_cancel (md: SMod.t) T msk (itr: itree _ T)
   (WF: SMod.cancellable md)
   (IMG: img_msk msk)
   (CALL: call_msk msk)
   :
-  @elim_rel tN (SMod.conc_sp_from md) T ε
+  @elim_rel (SMod.conc_sp_from md) T ε
     (inline_body (sandboxed_prog (SMod.to_mod ∅ (SMod.cancel md))) 
-      (SB.sandbox msk (SModTr.trans ∅ sN stid itr)))
+      (SB.sandbox msk (SModTr.trans ∅ itr)))
     (inline_body (sandboxed_prog (SMod.to_mod (SMod.conc_sp_from md) md)) 
-      (SB.sandbox msk (SModTr.trans (SMod.conc_sp_from md) tN ttid itr))).
+      (SB.sandbox msk (SModTr.trans (SMod.conc_sp_from md) itr))).
 Proof using.
-  ginit. revert IMG CALL. revert T itr sN stid ttid msk. gcofix CIH. i.
+  ginit. revert IMG CALL. revert T itr msk. gcofix CIH. i.
   dup WF. red in WF. dup IMG. red in IMG. des.
   assert (CASE:= case_itrH itr). des; subst.
   - rewrite !SRed.ret !SBRed.ret !MIRed.ret. estep 1.
@@ -659,7 +656,7 @@ Proof using.
       destruct (msk _ (subevent _ GetTid)) eqn:Y; cycle 1.
       { ss. rewrite SBRed.vis Y vis_trigger bind_bind MIRed.core. estep 1. }
       rewrite !MIRed.bind !SBRed_HoareGetTid // !MIRed_HoareGetTid.
-      gstep. rewrite (HoareGetTidE_indep stid ttid).
+      gstep.
       eapply elim_rel_gettid; eauto.
       i; s. edone.
     }
@@ -717,7 +714,7 @@ Section CancelDef.
       (MAIN: sp !! speckey_entry = Some (fspec_simple PQ))
       (RET: tid = 0 -> k = main_post PQ N mm)
       (TEQ: cid = tid)
-      (REL: elim_rel N sp r_diff itrS itrT)
+      (REL: elim_rel sp r_diff itrS itrT)
       (SRC: src = ModTr.trans itrS)
       (TGT: tgt = ModTr.trans itrT >>= k) :
      thread_rel PQ N mm sp cid tid r_diff src tgt
@@ -727,11 +724,11 @@ Section CancelDef.
      fspo = Some (@fspec_mk _ m pre post) →
      src = ModTr.trans (tau;; tau;; itrS) →
      tgt = ModTr.trans (
-       '(N', tid, m, varg):_ <- elim_spawnee_precond pre arg;;
-       vret <- bd N' tid varg;;
-       elim_spawnee_postcond post N' tid m vret) →
-     (Own r_diff ⊢ |==> pre (N, tid) x varg arg)%I →
-     elim_rel N sp ε itrS (bd N tid varg) →
+       '(m, varg):_ <- elim_spawnee_precond pre arg;;
+       vret <- bd varg;;
+       elim_spawnee_postcond post m vret) →
+     (Own r_diff ⊢ |==> pre x varg arg)%I →
+     elim_rel sp ε itrS (bd varg) →
      thread_rel PQ N mm sp cid tid r_diff src tgt
   | thread_rel_yield src tgt r_diff tid itrS itrT (k: Any.t → itree lmodE Any.t) :
      sp !! speckey_entry = Some (fspec_simple PQ) →
@@ -739,7 +736,7 @@ Section CancelDef.
      cid ≠ tid →
      src = ModTr.trans (tau;; itrS) →
      tgt = ModTr.trans (tau;; trigger (Assume (TID(tid) ∗ YIELD(tid) ∗ winv(↑N, ↑N)));;; tau;; itrT) >>= k →
-     elim_rel N sp ε itrS itrT →
+     elim_rel sp ε itrS itrT →
      thread_rel PQ N mm sp cid tid r_diff src tgt
   .
   
@@ -810,7 +807,7 @@ Section CancelDef.
       (x1 : tgts !! cid = Some (x <- ModTr.trans (x <- it_tgt;; ktrT x);; k x))
       (x2 : rs_diff !! cid = Some ε)
       (RET : cid = 0 → k = main_post PQ N mm)
-      (KTR : ∀ x, paco4 (elim_rel_def N sp) bot4 Any.t ε (ktrS x) (ktrT x)),
+      (KTR : ∀ x, paco4 (elim_rel_def sp) bot4 Any.t ε (ktrS x) (ktrT x)),
 
   gpaco7 _gsim (cpn7 _gsim) bot7 r (Any.t * Any.t)%type 
     (Any.t * Any.t)%type cancel_eq ps pt
