theories/modules/FSpec.v
@@ -4,8 +4,8 @@ From iris.proofmode Require Import proofmode.
 (* Function specifications *)
 Record fspec `{Σ : GRA} : Type := fspec_mk {
   meta : Type;
-  precond : (namespace * nat) → meta → Any.t → Any.t → iProp Σ;
-  postcond : (namespace * nat) → meta → Any.t → Any.t → iProp Σ;
+  precond : meta → Any.t → Any.t → iProp Σ;
+  postcond : meta → Any.t → Any.t → iProp Σ;
 }.
 Arguments fspec_mk {Σ meta} precond postcond.
 
@@ -14,18 +14,18 @@ Section fspec.
 
   Definition fspec_trivial : fspec :=
     @fspec_mk _ unit
-      (λ _ _ varg arg, ⌜varg = arg⌝%I)
-      (λ _ _ vret ret, ⌜vret = ret⌝%I).
+      (λ _ varg arg, ⌜varg = arg⌝%I)
+      (λ _ vret ret, ⌜vret = ret⌝%I).
 
   Definition fspec_bot : fspec :=
     @fspec_mk _ unit
-      (λ _ _ varg arg, True%I)
-      (λ _ _ vret ret, False%I).
+      (λ _ varg arg, True%I)
+      (λ _ vret ret, False%I).
 
   Definition fspec_top : fspec :=
     @fspec_mk _ False
-      (λ _ _ varg arg, False%I)
-      (λ _ _ vret ret, True%I).
+      (λ _ varg arg, False%I)
+      (λ _ vret ret, True%I).
 
   Definition fspec_flat (fspo : option fspec) : fspec :=
     or_else fspo fspec_trivial.
@@ -43,20 +43,20 @@ Section fspec.
 
   Definition fspec_simple {X} (PQ : X → (Any.t → iProp Σ) * (Any.t → iProp Σ)) : fspec :=
     fspec_mk
-      (λ A x varg arg, ⌜varg = arg⌝ ∗ (PQ x).1 varg)%I
-      (λ A x vret ret, ⌜vret = ret⌝ ∗ (PQ x).2 vret)%I.
+      (λ x varg arg, ⌜varg = arg⌝ ∗ (PQ x).1 varg)%I
+      (λ x vret ret, ⌜vret = ret⌝ ∗ (PQ x).2 vret)%I.
 
   Definition fspec_virtual
       {M VA VR : Type}
       (DPQ : M → (VA → Any.t → iProp Σ) * (VR → Any.t → iProp Σ)) :=
     fspec_mk
-      (λ _ x varg arg, (∃ (va : VA), ⌜varg = va↑⌝ ∗ (DPQ x).1 va arg)%I)
-      (λ _ x vret ret, (∃ (vr : VR), ⌜vret = vr↑⌝ ∗ (DPQ x).2 vr ret)%I).
+      (λ x varg arg, (∃ (va : VA), ⌜varg = va↑⌝ ∗ (DPQ x).1 va arg)%I)
+      (λ x vret ret, (∃ (vr : VR), ⌜vret = vr↑⌝ ∗ (DPQ x).2 vr ret)%I).
 
   Definition app_fspec (fspecs : list fspec) : fspec :=
     @fspec_mk _ { i : nat & meta (nth i fspecs fspec_top) }
-      (λ A '(existT i meta_i), precond (nth i fspecs fspec_top) A meta_i)
-      (λ A '(existT i meta_i), postcond (nth i fspecs fspec_top) A meta_i).
+      (λ '(existT i meta_i), precond (nth i fspecs fspec_top) meta_i)
+      (λ '(existT i meta_i), postcond (nth i fspecs fspec_top) meta_i).
 
   (* Simple fspecs. Assumes virtual arg = physical arg *)
   (* Record fspecS : Type := mk_fspecS {
@@ -82,13 +82,13 @@ Section fspec.
 
   (* Takes fspecS, generates inlinable specification *)
   Definition atomic_body
-    (fsp : fspec) (body : (namespace * nat) → meta fsp → Any.t → itree crisE Any.t)
+    (fsp : fspec) (body : meta fsp → Any.t → itree crisE Any.t)
     : Any.t → itree crisE Any.t :=
   λ arg,
-    x <- trigger (Take ((namespace * nat) * meta fsp));;
-    trigger (Assume ((precond fsp) x.1 x.2 arg arg));;;
-    ret <- body x.1 x.2 arg;;
-    trigger (Guarantee ((postcond fsp) x.1 x.2 ret ret));;;
+    x <- trigger (Take (meta fsp));;
+    trigger (Assume ((precond fsp) x arg arg));;;
+    ret <- body x arg;;
+    trigger (Guarantee ((postcond fsp) x ret ret));;;
     Ret ret.
 
   (* Definition lat_img_body
@@ -136,17 +136,17 @@ Section fspec.
         if P1 ⊢ P0 and Q0 ⊢ Q1 and { P0 } e { Q0 } then { P1 } e { Q1 }
       Therefore (P0, Q0) is stronger than (P1, Q1) if P1 ⊢ P0 and Q0 ⊢ Q1 *)
   Definition fspec_imply (fsp0 fsp1 : fspec) : Prop :=
-    ∀ Ntid, ∀ x1, ∃ x0,
-      (∀ varg arg, (precond fsp1 Ntid x1 varg arg ⊢ |==> precond fsp0 Ntid x0 varg arg)) ∧
-      (∀ vret ret, (postcond fsp0 Ntid x0 vret ret ⊢ |==> postcond fsp1 Ntid x1 vret ret)).
+    ∀ x1, ∃ x0,
+      (∀ varg arg, (precond fsp1 x1 varg arg ⊢ |==> precond fsp0 x0 varg arg)) ∧
+      (∀ vret ret, (postcond fsp0 x0 vret ret ⊢ |==> postcond fsp1 x1 vret ret)).
 
   Global Program Instance fspec_imply_PreOrder : PreOrder fspec_imply.
   Next Obligation.
   Proof using. ii; eexists; esplits; ii; et. Qed.
   Next Obligation.
   Proof using.
-    intros x y z Hxy Hyz Ntid mz; hexploit (Hyz Ntid mz); intros [my [Hzy Hyz']].
-    hexploit (Hxy Ntid my); intros [mx [Hyx Hxy']]; exists mx; split.
+    intros x y z Hxy Hyz mz; hexploit (Hyz mz); intros [my [Hzy Hyz']].
+    hexploit (Hxy my); intros [mx [Hyx Hxy']]; exists mx; split.
     { ii; rewrite Hzy Hyx; iIntros ">>$ //". }
     { ii; rewrite Hxy' Hyz'; iIntros ">>$ //". }
   Qed.
@@ -191,10 +191,10 @@ End fspec.
 Section fspec_WINV.
   Context `{!crisG Γ Σ α β τ _S _I}.
 
-  Definition fspec_winv (fsp : fspec) : fspec :=
-    fspec_mk (meta := meta fsp)
-      (λ '(N, stid) x varg arg, winv (↑N, ↑N) ∗ precond fsp (N, stid) x varg arg)%I
-      (λ '(N, stid) x vret ret, winv (↑N, ↑N) ∗ postcond fsp (N, stid) x vret ret)%I.
+  Definition fspec_winv (N : namespace) (fsp : fspec) : fspec :=
+    fspec_mk (meta := namespace * meta fsp)
+      (λ '(N, x) varg arg, winv (↑N, ↑N) ∗ precond fsp x varg arg)%I
+      (λ '(N, x) vret ret, winv (↑N, ↑N) ∗ postcond fsp x vret ret)%I.
 
   Definition icond_winv (E : coPset) (I : iProp Σ) : iProp Σ :=
     winv (E, E) ∗ I.
